Logic/Modal/Basic/Soundness.lean
@@ -8,32 +8,28 @@ namespace Hilbert
 
 open Formula
 
-variable {α β : Type u} {p : Formula α} (f : Frame β)
+variable {α β : Type u}
 
-lemma LogicK.sounds' {p : Formula α} (f : Frame β) : (⊢ᴴ(𝗞) p) → (⊧ᶠ[f] p) := by
-  intro h;
-  simp [ProofH] at h;
-  sorry;
-  -- TODO: この帰納法が回ればいいのだが上手くいってない
-  -- induction h using DerivationH.rec' <;> simp;
-
-  /--
-  induction h.some using bbb <;> try {simp_all [satisfies_imp, satisfies];}
+theorem LogicK.sounds (Γ : Set (Formula α)) (p : Formula α) (f : Frame β) (d : Γ ⊢ᴴ(𝐊) p) : (Γ ⊨ᶠ[f] p) := by
+  induction d <;> try {simp_all [satisfies_imp, satisfies];}
+  case wk _ _ _ hΓΔ _ ih =>
+    apply FrameConsequence.preserveWeakening hΓΔ ih;
+  case maxm Γ p ih =>
+    let ⟨_, ⟨_, hq⟩⟩ := ih; rw [←hq];
+    apply FrameConsequence.preserveAxiomK;
   case disj₃ p q r =>
     intro V w;
     by_cases (w ⊧ˢ[⟨f, V⟩] p) <;> simp_all [satisfies_imp, satisfies];
-  case modus_ponens p q d₁ d₂ ih₁ ih₂ => exact frames_ModusPonens (ih₁ ⟨d₁⟩) (ih₂ ⟨d₂⟩);
-  case necessitation p d ih => exact frames_Necessitation (ih ⟨d⟩);
-  -/
+  case necessitation _ p _ ih =>
+    exact FrameConsequence.preserveNecessitation ih;
 
-lemma LogicK.sounds {p : Formula α} (f : Frame β) : (h : ⊢ᴴ(𝗞)! p) → (⊧ᶠ[f] p) := by
-  intro h; exact sounds' f h.some;
+lemma LogicK.sounds' {p : Formula α} (f : Frame β) (h : ⊢ᴴ(𝐊)! p) : (⊧ᶠ[f] p) := by
+  simpa using sounds ∅ p f h.some;
 
-theorem LogicK.unprovable_bot : (⊬ᴴ(𝗞)! (⊥ : Formula α)) := by
+theorem LogicK.unprovable_bot {f : Frame β} : (⊬ᴴ(𝐊)! (⊥ : Formula α)) := by
   by_contra hC; simp at hC;
-  have w := f.nonempty.some;
-  suffices ⊧ᶠ[f] (⊥ : Formula α) by simp_all [satisfies_bot]; exact this w;
-  exact sounds f hC;
+  suffices h : ⊧ᶠ[f] (⊥ : Formula α) by exact frames_bot h;
+  exact sounds' f hC;
 
 end Hilbert
 
